DinD: Move Values out of interpreter

Source/DafnyCompilers/Semantics.dfy
@@ -1,71 +1,6 @@
 include "CompilerCommon.dfy"
 include "Library.dfy"
-
-module Values {
-  import Lib.Math
-  import opened Lib.Datatypes
-  import Ty = DafnyCompilerCommon.AST.Types
-
-  datatype Value =
-    | Bool(b: bool)
-    | Char(c: char)
-    | Int(i: int)
-    | Real(r: real)
-    | BigOrdinal(o: ORDINAL)
-    | BitVector(value: int)
-    | Map(m: map<Value, Value>)
-    | MultiSet(ms: multiset<Value>)
-    | Seq(sq: seq<Value>)
-    | Set(st: set<Value>)
-  {
-    predicate method HasType(ty: Ty.Type) {
-      match (this, ty) // FIXME tests on other side
-        case (Bool(b), Bool()) => true
-        case (Char(c), Char()) => true
-        case (Int(i), Int()) => true
-        case (Real(r), Real()) => true
-        case (BigOrdinal(o), BigOrdinal()) => true
-        case (BitVector(value), BitVector(width)) =>
-          0 <= value < Math.IntPow(2, width)
-        case (Map(m), Collection(true, Map(kT), eT)) =>
-          forall x | x in m :: x.HasType(kT) && m[x].HasType(eT)
-        case (MultiSet(ms), Collection(true, MultiSet, eT)) =>
-          forall x | x in ms :: x.HasType(eT)
-        case (Seq(sq), Collection(true, Seq, eT)) =>
-          forall x | x in sq :: x.HasType(eT)
-        case (Set(st), Collection(true, Set, eT)) =>
-          forall x | x in st :: x.HasType(eT)
-
-        case (Bool(b), _) => false
-        case (Char(c), _) => false
-        case (Int(i), _) => false
-        case (Real(r), _) => false
-        case (BigOrdinal(o), _) => false
-        case (BitVector(value), _) => false
-        case (Map(m), _) => false
-        case (MultiSet(ms), _) => false
-        case (Seq(sq), _) => false
-        case (Set(st), _) => false
-    }
-
-    function method Cast(ty: Ty.Type) : (v: Option<Value>)
-      ensures v.Some? ==> HasType(ty)
-    {
-      if HasType(ty) then Some(this) else None
-    }
-  }
-
-  type T = Value
-
-  datatype TypedValue = Value(ty: Ty.Type, v: T) {
-    predicate Wf() { v.HasType(ty) }
-  }
-
-  // FIXME how do we define the interpreter to support :| without committing to a single interpretation of :|?
-  // NOTE: Maybe tag each syntactic :| with a distinct color and add the color somehow into the Dafny-side :| used to implement it.  Pro: it allows inlining.
-}
-
-type Value = Values.T
+include "Values.dfy"
 
 module Interp {
   import opened Lib.Datatypes
@@ -167,7 +102,7 @@ module Interp {
     requires SupportsInterp(e)
     decreases e, 0
   {
-    Predicates.AllImpliesChildren(e, SupportsInterp1); // DISCUSS
+    Predicates.Deep.AllImpliesChildren(e, SupportsInterp1);
     match e {
       case Literal(lit) => Success(OK(InterpLiteral(lit), ctx))
       case Apply(aop, args: seq<Expr>) =>
